A few 'preservation' results of the SoA transformation proved.

TrSoA.v
@@ -24,7 +24,7 @@ Open Scope Z_scope.
 Record soa_tr := make_soa_tr {
   soa_tr_array_name : typvar;
   soa_tr_struct_name : typvar;
-  soa_tr_struct_fields : set field;
+  soa_tr_struct_fields : map field typ;
   soa_tr_array_size : size
 }.
 
@@ -33,13 +33,12 @@ Notation make_soa_tr' := make_soa_tr.
 (** Checking if the transformation is acceptable *)
 
 Inductive soa_tr_ok : soa_tr -> typdefctx -> Prop :=
-  | soa_tr_ok_intros : forall Ta Ts fs K Tfs st C,
-      st = make_soa_tr Ta Ts fs K ->
+  | soa_tr_ok_intros : forall Ta Ts Tfs K st C,
+      st = make_soa_tr Ta Ts Tfs K ->
       Ta \indom C ->
       Ts \indom C ->
       C[Ta] = typ_array (typ_var Ts) (Some K) ->
       C[Ts] = typ_struct Tfs ->
-      fs = dom Tfs ->
       K > 0%Z ->
       (forall Tv,
         Tv \indom C ->
@@ -58,14 +57,13 @@ Inductive soa_tr_ok : soa_tr -> typdefctx -> Prop :=
 (** Transformation of typdefctxs: C ~ |C| *)
 
 Inductive tr_typdefctx (st:soa_tr) : typdefctx -> typdefctx -> Prop :=
-  | tr_typdefctx_intro : forall Ta Ts fs K Tfs Tfs' C C',
-      st = make_soa_tr Ta Ts fs K ->
+  | tr_typdefctx_intro : forall Ta Ts Tfs K Tfs' C C',
+      st = make_soa_tr Ta Ts Tfs K ->
       dom C' \u \{Ta} = dom C ->
       Ta \notindom C' ->
       C[Ta] = typ_array (typ_var Ts) (Some K) ->
       C[Ts] = typ_struct Tfs ->
       C'[Ts] = typ_struct Tfs' ->
-      fs = dom Tfs ->
       dom Tfs = dom Tfs' ->
       (forall f,
         f \indom Tfs ->
@@ -81,13 +79,13 @@ Inductive tr_typdefctx (st:soa_tr) : typdefctx -> typdefctx -> Prop :=
 Inductive tr_accesses (st:soa_tr) : accesses -> accesses -> Prop :=
   | tr_accesses_nil :
       tr_accesses st nil nil
-  | tr_accesses_soa : forall Ta Ts fs K f T i a0 a1 π a0' a1' π',
+  | tr_accesses_soa : forall Ta Ts Tfs K f i a0 a1 π a0' a1' π',
       tr_accesses st π π' ->
-      st = make_soa_tr Ta Ts fs K ->
-      a0 = access_array (typ_var Ts) i ->
-      a1 = access_field T f ->
-      a0' = access_field (typ_array T (Some K)) f ->
-      a1' = access_array T i ->
+      st = make_soa_tr Ta Ts Tfs K ->
+      a0 = access_array (typ_var Ta) i ->
+      a1 = access_field (typ_var Ts) f ->
+      a0' = access_field (typ_var Ts) f ->
+      a1' = access_array (typ_array Tfs[f] (Some K)) i ->
       tr_accesses st (a0::a1::π) (a0'::a1'::π')
   | tr_accesses_array_other : forall π π' T i,
       T <> typ_var (soa_tr_array_name st) ->
@@ -113,10 +111,11 @@ Inductive tr_val (st:soa_tr) : val -> val -> Prop :=
   | tr_val_abstract_ptr : forall l π π',
       tr_accesses st π π' ->
       tr_val st (val_abstract_ptr l π) (val_abstract_ptr l π')
-  | tr_val_array_tiling : forall fs K Ta a Ts s',
-      st = make_soa_tr Ta Ts fs K ->
+  | tr_val_array_tiling : forall Tfs K Ta a Ts s',
+      st = make_soa_tr Ta Ts Tfs K ->
+      dom s' = dom Tfs ->
       (forall f a' T,
-        f \in fs ->
+        f \indom Tfs ->
             s'[f] = val_array (typ_array T (Some K)) a'
         /\  (forall s i,
               index a' i ->
@@ -139,9 +138,9 @@ Inductive tr_val (st:soa_tr) : val -> val -> Prop :=
 
 (* Transformation used in the struct cases to avoid repetition. *)
 
-Inductive tr_array_op (st:soa_tr) : trm -> trm -> Prop :=
-  | tr_array_access_soa : forall Ta Ts fs K T f t ti ts ta ts' ta',
-      st = make_soa_tr Ta Ts fs K ->
+Inductive tr_struct_op (st:soa_tr) : trm -> trm -> Prop :=
+  | tr_struct_access_soa : forall Ta Ts Tfs K T f t ti ts ta ts' ta',
+      st = make_soa_tr Ta Ts Tfs K ->
       (* Initial term is ts: &(t[i]->f) *)
       ta = trm_app (prim_struct_access (typ_var Ts) f) (ts::nil) ->
       ts = trm_app (prim_array_access T) (t::ti::nil) ->
@@ -149,9 +148,9 @@ Inductive tr_array_op (st:soa_tr) : trm -> trm -> Prop :=
       ts' = trm_app (prim_array_access (typ_var Ta)) (ta'::ti::nil) ->
       ta' = trm_app (prim_struct_access T f) (t::nil) ->
       (* Result. *)
-      tr_array_op st ta ts'
-  | tr_array_get_soa : forall Ta Ts fs K T f t ti ts ta ts' ta',
-      st = make_soa_tr Ta Ts fs K ->
+      tr_struct_op st ta ts'
+  | tr_struct_get_soa : forall Ta Ts Tfs K T f t ti ts ta ts' ta',
+      st = make_soa_tr Ta Ts Tfs K ->
       (* Initial term is ts: t[i].f *)
       ta = trm_app (prim_struct_get (typ_var Ts) f) (ts::nil) ->
       ts = trm_app (prim_array_get T) (t::ti::nil) ->
@@ -159,15 +158,15 @@ Inductive tr_array_op (st:soa_tr) : trm -> trm -> Prop :=
       ts' = trm_app (prim_array_get (typ_var Ta)) (ta'::ti::nil) ->
       ta' = trm_app (prim_struct_get T f) (t::nil) ->
       (* Result. *)
-      tr_array_op st ta ts'
-  | tr_array_access_other : forall Ts T f ts,
+      tr_struct_op st ta ts'
+  | tr_struct_access_other : forall Ts T f ts,
       Ts = soa_tr_struct_name st ->
       T <> (typ_var Ts) ->
-      tr_array_op st (trm_app (prim_struct_access T f) ts) (trm_app (prim_struct_access T f) ts)
-  | tr_array_get_other : forall Ts T f ts,
+      tr_struct_op st (trm_app (prim_struct_access T f) ts) (trm_app (prim_struct_access T f) ts)
+  | tr_struct_get_other : forall Ts T f ts,
       Ts = soa_tr_struct_name st ->
       T <> (typ_var Ts) ->
-      tr_array_op st (trm_app (prim_struct_get T f) ts) (trm_app (prim_struct_get T f) ts).
+      tr_struct_op st (trm_app (prim_struct_get T f) ts) (trm_app (prim_struct_get T f) ts).
 
 (** Transformation of terms: t ~ |t| *)
 
@@ -193,7 +192,7 @@ Inductive tr_trm (st:soa_tr) : trm -> trm -> Prop :=
   | tr_trm_array : forall t1' op t1 tr,
       is_struct_op op ->
       tr_trm st t1 t1' ->
-      tr_array_op st (trm_app op (t1'::nil)) tr ->
+      tr_struct_op st (trm_app op (t1'::nil)) tr ->
       tr_trm st (trm_app op (t1::nil)) tr
   (* Args *)
   | tr_trm_args1 : forall op t1 t1',
@@ -207,22 +206,184 @@ Inductive tr_trm (st:soa_tr) : trm -> trm -> Prop :=
 
 (** Transformation of stacks: S ~ |S| *)
 
-Inductive tr_stack_item (tt:tiling_tr) : (var * val) -> (var * val) -> Prop :=
+Inductive tr_stack_item (st:soa_tr) : (var * val) -> (var * val) -> Prop :=
   | tr_stack_item_intro : forall x v v',
-      tr_val tt v v' -> 
-      tr_stack_item tt (x, v) (x, v').
+      tr_val st v v' -> 
+      tr_stack_item st (x, v) (x, v').
 
-Inductive tr_stack (tt:tiling_tr) : stack -> stack -> Prop :=
+Inductive tr_stack (st:soa_tr) : stack -> stack -> Prop :=
   | tr_stack_intro : forall S S',
-      LibList.Forall2 (tr_stack_item tt) S S' ->
-      tr_stack tt S S'.
+      LibList.Forall2 (tr_stack_item st) S S' ->
+      tr_stack st S S'.
 
 (** Transformation of states: m ~ |m| *)
 
-Inductive tr_state (tt:tiling_tr) : state -> state -> Prop :=
+Inductive tr_state (st:soa_tr) : state -> state -> Prop :=
   | tr_state_intro : forall m m',
       dom m = dom m' ->
       (forall l,
         l \indom m ->
-        tr_val tt m[l] m'[l]) ->
-      tr_state tt m m'.
+        tr_val st m[l] m'[l]) ->
+      tr_state st m m'.
+
+
+(* ********************************************************************** *)
+(* * Preservation of semantics proof. *)
+
+Lemma stack_lookup_tr : forall st S S' x v,
+  tr_stack st S S' ->
+  Ctx.lookup x S = Some v -> 
+    exists v', 
+       Ctx.lookup x S' = Some v' 
+    /\ tr_val st v v'.
+Proof.
+  introv HS Hx. inverts HS as HS. induction HS.
+  { inverts Hx. }
+  { inverts H as Hv. inverts Hx as Hx. case_if in Hx.
+    { inverts Hx. exists v'. splits*. unfolds. case_if*. }
+    { forwards (v''&Hx'&Hv''): IHHS Hx. exists v''.
+      splits*. unfolds. case_if. fold Ctx.lookup. auto. } }
+Qed.
+
+Lemma tr_stack_add : forall st z v S v' S',
+  tr_stack st S S' ->
+  tr_val st v v' ->
+  tr_stack st (Ctx.add z v S) (Ctx.add z v' S').
+Proof.
+  introv HS Hv. constructors~. inverts HS.
+  unfolds Ctx.add. destruct* z.
+  applys~ Forall2_cons. constructors~.
+Qed.
+
+Lemma is_basic_tr : forall st v1 v2,
+  tr_val st v1 v2 ->
+  is_basic v1 ->
+  is_basic v2.
+Proof.
+  introv Htr Hv1. induction Htr;
+  try solve [ inverts Hv1 ];
+  constructors~.
+Qed.
+
+Lemma not_tr_val_error : forall st v1 v2,
+  tr_val st v1 v2 ->
+  ~ is_error v2.
+Proof.
+  introv Hv He. unfolds is_error.
+  destruct* v2. inverts Hv.
+Qed.
+
+Lemma not_is_val_tr : forall st t1 t2,
+  tr_trm st t1 t2 ->
+  ~ is_val t1 ->
+  ~ is_val t2.
+Proof.
+  introv Htr Hv. induction Htr; introv HN;
+  try solve [ subst ; inverts HN ].
+  forwards*: Hv. inverts H0 as; inverts HN.
+Qed.
+
+Lemma not_is_error_tr : forall gt v1 v2,
+  tr_val gt v1 v2 ->
+  ~ is_error v2.
+Proof.
+  introv Htr. induction Htr; introv HN;
+  try solve [ subst ; inverts HN ].
+Qed.
+
+Lemma not_is_uninitialized_tr : forall st v v',
+  tr_val st v v' -> 
+  ~ is_uninitialized v ->
+  ~ is_uninitialized v'.
+Proof.
+  introv Htr Hu HN. induction Htr; subst; inverts HN as.
+  { applys* Hu. constructors. }
+  { introv (f&Hfin&Hus'f).
+    applys~ Hu. forwards* (Hs'f&Htr): H1 f a.
+    { rewrite~ H0 in Hfin. } 
+    rewrite Hs'f in Hus'f.
+    inverts Hus'f. constructors~. }
+  { introv (i&Hi&Hua'i).
+    asserts Hi': (index a i).
+    { rewrite index_eq_index_length in *. rewrite~ H0. }
+    applys* H2. introv HN. applys~ Hu.
+    constructors. exists i. splits~. }
+  { introv (f&Hfin&Hus'f).
+    asserts Hf': (f \indom s).
+    { rewrite~ H. }
+    applys* H1. introv HN. applys~ Hu. constructors.
+    exists f. splits~. }
+Unshelve. typeclass.
+Qed.
+
+(* Functional results. *)
+
+Theorem functional_tr_accesses : forall st π π1 π2,
+  tr_accesses st π π1 ->
+  tr_accesses st π π2 ->
+    π1 = π2.
+Proof.
+  introv H1 H2. gen π2. induction H1; intros.
+  { inverts~ H2. }
+  { inverts_head tr_accesses; tryfalse.
+    { inverts_head access_array.
+      inverts_head access_field.
+      inverts_head make_soa_tr'.
+      subst. repeat fequals.
+      applys~ IHtr_accesses. }
+    { subst. simpls. inverts_head access_array. false. } }
+  { inverts H2; try solve [ simpls; false ].
+    fequals. applys~ IHtr_accesses. }
+  { inverts H2; try solve [ simpls; false ].
+    fequals. applys~ IHtr_accesses. }
+Qed.
+
+Theorem functional_tr_val : forall st v v1 v2,
+  tr_val st v v1 ->
+  tr_val st v v2 ->
+  v1 = v2.
+Proof using.
+Admitted.
+
+Lemma tr_accesses_inj : forall C st π π1 π2,
+  soa_tr_ok st C ->
+  wf_accesses C π1 ->
+  wf_accesses C π2 ->
+  tr_accesses st π1 π ->
+  tr_accesses st π2 π ->
+    π1 = π2.
+Proof.
+Admitted.
+
+Lemma tr_val_inj : forall C st v v1 v2,
+  soa_tr_ok st C ->
+  is_basic v1 ->
+  is_basic v2 ->
+  wf_val C v1 ->
+  wf_val C v2 ->
+  tr_val st v1 v ->
+  tr_val st v2 v ->
+  v1 = v2.
+Proof.
+  introv Hok HBv1 HBv2 Hwfv1 Hwfv2 Hv1 Hv2. gen C v2. induction Hv1; intros;
+  try solve [ inverts Hv2; repeat fequals*; subst; simpls; tryfalse* ].
+  { inverts Hv2 as Hπ. repeat fequals*.
+    inverts Hwfv1 as HRφ1. inverts Hwfv2 as HRφ2.
+    applys* tr_accesses_inj. }
+Qed.
+
+Lemma tr_val_inj_cp : forall C st v1 v2 v1' v2',
+  soa_tr_ok st C ->
+  is_basic v1 ->
+  is_basic v2 ->
+  wf_val C v1 ->
+  wf_val C v2 ->
+  tr_val st v1 v1' ->
+  tr_val st v2 v2' ->
+  v1 <> v2 ->
+  v1' <> v2'.
+Proof.
+  introv Hok HBv1 HBv2 HTv1 HTv2 Hv1 Hv2 Hneq HN. subst.
+  forwards*: tr_val_inj Hok HTv1 HTv2 Hv1.
+Qed.
+
